formal/inference/EFSM_Dot.thy
@@ -74,7 +74,7 @@ fun gexp2dot :: "gexp \<Rightarrow> String.literal" where
   "gexp2dot (GExp.Bc True) = (STR ''True'')" |
   "gexp2dot (GExp.Bc False) = (STR ''False'')" |
   "gexp2dot (GExp.Eq a1 a2) = (aexp2dot a1)+STR '' = ''+(aexp2dot a2)" |
-  "gexp2dot (GExp.Lt a1 a2) = (aexp2dot a1)+STR '' &lt; ''+(aexp2dot a2)" |
+  "gexp2dot (GExp.Gt a1 a2) = (aexp2dot a1)+STR '' &gt; ''+(aexp2dot a2)" |
   "gexp2dot (GExp.In v l) = (vname2dot v)+STR ''&isin;{''+(join (map value2dot l) STR '', '')+STR ''}''" |
   "gexp2dot (Nor g1 g2) = STR ''!(''+(gexp2dot g1)+STR ''&or;''+(gexp2dot g2)+STR '')''" |
   "gexp2dot (Null v) = (aexp2dot v)+STR '' = NULL''"
